more opentitan-like acorn circuit, and proofs

silveroak-opentitan/aes/Acorn/AES256Equivalence.v
@@ -14,9 +14,14 @@
 (* limitations under the License.                                           *)
 (****************************************************************************)
 
+Require Import Coq.Arith.PeanoNat.
 Require Import Coq.Vectors.Vector.
+Require Import Coq.Lists.List.
+Require Import coqutil.Tactics.destr.
 Require Import ExtLib.Structures.Monads.
+Require Import Cava.BitArithmetic.
 Require Import Cava.ListUtils.
+Require Import Cava.Tactics.
 Require Import Cava.VectorUtils.
 Require Import Cava.Acorn.Acorn.
 Require Import Cava.Acorn.MonadFacts.
@@ -25,12 +30,17 @@ Require Import Cava.Acorn.Identity.
 Require Import AesSpec.AES256.
 Require Import AesSpec.StateTypeConversions.
 Require Import AesSpec.CipherProperties.
+Require Import AesSpec.ExpandAllKeys.
 Require Import AcornAes.AddRoundKey.
 Require Import AcornAes.AddRoundKeyEquivalence.
 Require Import AcornAes.CipherRound.
 Require Import AcornAes.CipherEquivalence.
 Require Import AcornAes.Common.
+Import ListNotations.
 Import Common.Notations.
+
+Local Notation round_constant := (Vec Bit 8) (only parsing).
+Local Notation round_index := (Vec Bit 4) (only parsing).
 
 Axiom sub_bytes : forall {signal} {semantics : Cava signal} {monad : Monad cava},
     signal Bit -> signal state -> cava (signal state).
@@ -38,6 +48,30 @@ Axiom shift_rows : forall {signal} {semantics : Cava signal} {monad : Monad cava
     signal Bit -> signal state -> cava (signal state).
 Axiom mix_columns : forall {signal} {semantics : Cava signal} {monad : Monad cava},
     signal Bit -> signal state -> cava (signal state).
+
+Axiom key_expand : forall {signal} {semantics : Cava signal} {monad : Monad cava},
+    signal Bit -> signal round_index -> signal key * signal round_constant ->
+    cava (signal key * signal round_constant).
+Axiom key_expand_spec : nat -> t bool 128 * t bool 8 -> t bool 128 * t bool 8.
+Axiom inv_key_expand_spec : nat -> t bool 128 * t bool 8 -> t bool 128 * t bool 8.
+
+(* convenience definition for converting to/from flat keys in key * round
+   constant pairs *)
+Definition flatten_key (kr : combType key * combType round_constant)
+  : t bool 128 * combType round_constant := (from_cols_bitvecs (fst kr), snd kr).
+Definition unflatten_key (kr : t bool 128 * combType round_constant)
+  : combType key * combType round_constant := (to_cols_bitvecs (fst kr), snd kr).
+Lemma flatten_unflatten kr : flatten_key (unflatten_key kr) = kr.
+Proof.
+  cbv [flatten_key unflatten_key]. destruct kr; cbn [fst snd].
+  autorewrite with conversions. reflexivity.
+Qed.
+Lemma unflatten_flatten kr : unflatten_key (flatten_key kr) = kr.
+Proof.
+  cbv [flatten_key unflatten_key]. destruct kr; cbn [fst snd].
+  autorewrite with conversions. reflexivity.
+Qed.
+Hint Rewrite @unflatten_flatten @flatten_unflatten using solve [eauto] : conversions.
 
 Axiom sub_bytes_equiv :
  forall st : t bool 128,
@@ -51,6 +85,12 @@ Axiom mix_columns_equiv :
   forall st : t bool 128,
     from_cols_bitvecs
       (combinational (mix_columns false (to_cols_bitvecs st))) = AES256.mix_columns st.
+Axiom key_expand_equiv :
+  forall (i : nat) (k : t (t (t bool 8) 4) 4 * t bool 8),
+    (i < 16)%nat ->
+    combinational (key_expand false (nat_to_bitvec_sized _ i) k)
+    = unflatten_key (key_expand_spec i (flatten_key k)).
+
 Axiom inv_sub_bytes_equiv :
  forall st : t bool 128,
    from_cols_bitvecs
@@ -63,42 +103,79 @@ Axiom inv_mix_columns_equiv :
   forall st : t bool 128,
     from_cols_bitvecs
       (combinational (mix_columns true (to_cols_bitvecs st))) = inv_mix_columns st.
+Axiom inv_key_expand_equiv :
+  forall (i : nat) (k : t (t (t bool 8) 4) 4 * t bool 8),
+    (i < 16)%nat ->
+    combinational (key_expand true (nat_to_bitvec_sized _ i) k)
+    = unflatten_key (inv_key_expand_spec i (flatten_key k)).
 
 Hint Resolve add_round_key_equiv sub_bytes_equiv shift_rows_equiv
      mix_columns_equiv inv_sub_bytes_equiv inv_shift_rows_equiv
      inv_mix_columns_equiv : subroutines_equiv.
 
 Definition full_cipher {signal} {semantics : Cava signal} {monad : Monad cava}
-  : signal Bit -> signal key -> signal key -> list (signal key) -> signal state
-    -> cava (signal state) :=
-  cipher sub_bytes shift_rows mix_columns add_round_key.
+           (num_rounds_regular round_0 : signal (Vec Bit 4))
+  : signal Bit -> signal key -> signal (Vec Bit 8) ->
+    list (signal (Vec Bit 4)) -> signal state -> cava (signal state) :=
+  cipher
+    (round_index:=Vec Bit 4) (round_constant:=Vec Bit 8)
+    sub_bytes shift_rows mix_columns add_round_key
+    (fun k => is_decrypt <- one ;; mix_columns is_decrypt k)
+    key_expand num_rounds_regular round_0.
 
 Lemma full_cipher_equiv
-      (is_decrypt : bool)
-      (first_key last_key : combType key) (middle_keys : list (combType key))
-      (input : combType state) :
+      (is_decrypt : bool) (first_rcon : t bool 8)
+      (first_key last_key : combType key)
+      middle_keys (input : combType state) :
+  let Nr := 14 in
+  let all_keys_and_rcons :=
+      all_keys (if is_decrypt
+                then (fun i k => unflatten_key (inv_key_expand_spec i (flatten_key k)))
+                else (fun i k => unflatten_key (key_expand_spec i (flatten_key k))))
+               Nr (first_key, first_rcon) in
+  let all_keys := List.map fst all_keys_and_rcons in
+  let round_indices := map (fun i => nat_to_bitvec_sized 4 i) (List.seq 0 (S Nr)) in
+  let middle_keys_flat :=
+      if is_decrypt
+      then List.map AES256.inv_mix_columns (List.map from_cols_bitvecs middle_keys)
+      else List.map from_cols_bitvecs middle_keys in
+  all_keys = (first_key :: middle_keys ++ [last_key])%list ->
   combinational
-    (full_cipher is_decrypt first_key last_key middle_keys input)
+    (full_cipher (nat_to_bitvec_sized _ Nr) (nat_to_bitvec_sized _ 0) is_decrypt
+                 first_key first_rcon round_indices input)
   = to_cols_bitvecs
       ((if is_decrypt then aes256_decrypt else aes256_encrypt)
-         (from_cols_bitvecs first_key) (from_cols_bitvecs last_key)
-         (List.map from_cols_bitvecs middle_keys) (from_cols_bitvecs input)).
+         (from_cols_bitvecs first_key) (from_cols_bitvecs last_key) middle_keys_flat
+         (from_cols_bitvecs input)).
 Proof.
-  cbv [full_cipher].
+  cbv [full_cipher]; intros.
 
   destruct is_decrypt.
   { (* decryption *)
-    rewrite inverse_cipher_equiv. cbv [aes256_decrypt].
+    erewrite inverse_cipher_equiv with (Nr:=14);
+      [ |  lazymatch goal with
+           | |- _ = (_ :: _ ++ [_])%list =>
+             erewrite ?all_keys_ext
+               by (intros; rewrite inv_key_expand_equiv by Lia.lia;
+                   instantiate_app_by_reflexivity); solve [eauto]
+           | _ => change (2^4)%nat with 16; (reflexivity || Lia.lia)
+           end .. ].
+
+    cbv [aes256_decrypt].
 
     (* Change key and state representations so they match *)
     erewrite equivalent_inverse_cipher_change_state_rep
       by eapply to_cols_bitvecs_from_cols_bitvecs.
     erewrite equivalent_inverse_cipher_change_key_rep
       with (projkey:=to_cols_bitvecs)
-           (middle_keys_alt:=List.map from_cols_bitvecs middle_keys)
-      by (apply to_cols_bitvecs_from_cols_bitvecs ||
-          (rewrite List.map_map; apply ListUtils.map_id_ext;
-           intros; autorewrite with conversions; reflexivity)).
+           (middle_keys_alt:=
+              List.map inv_mix_columns (List.map from_cols_bitvecs middle_keys))
+           (first_key_alt:=from_cols_bitvecs first_key)
+           (last_key_alt:=from_cols_bitvecs last_key)
+      by (try apply to_cols_bitvecs_from_cols_bitvecs;
+          rewrite !List.map_map; apply List.map_ext;
+          intros; rewrite <-inv_mix_columns_equiv;
+          autorewrite with conversions; reflexivity).
 
     (* Prove that ciphers are equivalent because all subroutines are
        equivalent *)
@@ -106,7 +183,16 @@ Proof.
     eapply equivalent_inverse_cipher_subroutine_ext;
       eauto with subroutines_equiv. }
   { (* encryption *)
-    rewrite cipher_equiv. cbv [aes256_encrypt].
+    erewrite cipher_equiv with (Nr:=14);
+      [ |  lazymatch goal with
+           | |- _ = (_ :: _ ++ [_])%list =>
+             erewrite ?all_keys_ext
+               by (intros; rewrite key_expand_equiv by Lia.lia;
+                   instantiate_app_by_reflexivity); solve [eauto]
+           | _ => change (2^4)%nat with 16; (reflexivity || Lia.lia)
+           end .. ].
+
+    cbv [aes256_encrypt].
 
     (* Change key and state representations so they match *)
     erewrite cipher_change_state_rep
@@ -138,19 +224,58 @@ Proof.
   autorewrite with conversions; reflexivity.
 Qed.
 
+(* TODO: define a downto/upto loop combinator and then prove the cipher in terms of that *)
 Lemma full_cipher_inverse
-      (first_key last_key : combType key) (middle_keys : list (combType key))
-      (input : combType state) :
-  let decrypt_middle_keys :=
-      List.map (fun k => combinational (mix_columns true k)) (List.rev middle_keys) in
+      (is_decrypt : bool) (first_rcon last_rcon : t bool 8)
+      (first_key last_key : combType key) (input : combType state) :
+  let Nr := 14 in
+  let all_keys_and_rcons :=
+      all_keys (fun i k => unflatten_key (key_expand_spec i (flatten_key k)))
+               Nr (first_key, first_rcon) in
+  let round_indices := map (fun i => nat_to_bitvec_sized 4 i) (List.seq 0 (S Nr)) in
+  (* last_key and last_rcon are correct *)
+  (exists keys, all_keys_and_rcons = keys ++ [(last_key, last_rcon)]) ->
+  (* inverse key expansion reverses key expansion *)
+  (forall i kr,
+      unflatten_key
+        (inv_key_expand_spec
+           (Nr - S i) (key_expand_spec i (flatten_key kr))) = kr) ->
   combinational
-    ((full_cipher false first_key last_key middle_keys >=>
-      full_cipher true last_key first_key decrypt_middle_keys) input) = input.
+    ((full_cipher (nat_to_bitvec_sized _ Nr) (nat_to_bitvec_sized _ 0)
+                  false first_key first_rcon round_indices >=>
+      full_cipher (nat_to_bitvec_sized _ Nr) (nat_to_bitvec_sized _ 0)
+                  true last_key last_rcon round_indices) input) = input.
 Proof.
-  cbv [mcompose]. simpl_ident.
-  rewrite !full_cipher_equiv.
+  cbv [mcompose]. intros [keys Hkeys] ?. simpl_ident.
+
+  (* extract the first key and middle keys to match full_cipher_equiv *)
+  lazymatch type of Hkeys with
+    ?all_keys = _ =>
+    let H := fresh in
+    assert (1 < length all_keys) as H by length_hammer;
+      rewrite Hkeys in H
+  end.
+  destruct keys; autorewrite with push_length in *; [ Lia.lia | ].
+  rewrite <-app_comm_cons in *.
+  let H := fresh in pose proof Hkeys as H; apply hd_all_keys in H; [ | Lia.lia ].
+  subst.
+
+  (* TODO(jadep): can ExpandAllKeys be improved to make this less awkward? *)
+  erewrite !full_cipher_equiv.
+  2:{
+    rewrite Hkeys. cbn [map]. rewrite map_app. cbn [map fst].
+    reflexivity. }
+  2:{
+    erewrite all_keys_inv_eq
+      by (intros; lazymatch goal with
+                  | |- _ = last _ _ => rewrite Hkeys, app_comm_cons, last_last; reflexivity
+                  | _ => cbv beta; autorewrite with conversions; auto
+                  end).
+    rewrite Hkeys. cbn [map rev]. rewrite map_app, rev_unit. cbn [map rev fst].
+    rewrite <-app_comm_cons. reflexivity. }
+
   autorewrite with conversions.
-  rewrite List.map_map, decrypt_middle_keys_equiv.
+  do 2 rewrite map_rev.
   rewrite aes256_decrypt_encrypt.
   autorewrite with conversions.
   reflexivity.
