silveroak-opentitan/aes/Acorn/CipherEquivalence.v
@@ -14,25 +14,50 @@
 (* limitations under the License.                                           *)
 (****************************************************************************)
 
+Require Import Coq.Arith.PeanoNat.
 Require Import Coq.Vectors.Vector.
+Require Import Coq.Lists.List.
+Require Import Coq.NArith.NArith.
+Require Import Coq.NArith.Ndigits.
+Import VectorNotations.
+Import ListNotations.
+
 Require Import ExtLib.Structures.Monads.
+Open Scope monad_scope.
+
+Require Import coqutil.Tactics.Tactics.
+Require Import Cava.BitArithmetic.
+Require Import Cava.NatUtils.
 Require Import Cava.ListUtils.
+Require Import Cava.VectorUtils.
+Require Import Cava.Tactics.
+
 Require Import Cava.Acorn.MonadFacts.
+Require Import Cava.Acorn.CombinationalProperties.
 Require Import Cava.Acorn.Acorn.
+Require Import Cava.Acorn.Identity.
 
 Require Import AesSpec.Cipher.
+Require Import AesSpec.CipherProperties.
+Require Import AesSpec.ExpandAllKeys.
+Require Import AesSpec.InterleavedCipher.
+Require Import AesSpec.InterleavedInverseCipher.
 Require Import AcornAes.CipherRound.
 
 Existing Instance CombinationalSemantics.
 
 Section WithSubroutines.
-  Local Notation byte := (t bool 8).
-  Local Notation state := (t (t byte 4) 4) (only parsing).
-  Local Notation key := (t (t byte 4) 4) (only parsing).
+  Local Notation byte := (Vector.t bool 8).
+  Local Notation state := (Vector.t (Vector.t byte 4) 4) (only parsing).
+  Local Notation key := (Vector.t (Vector.t byte 4) 4) (only parsing).
+  Local Notation round_index := (Vector.t bool 4) (only parsing).
+  Local Notation round_constant := byte (only parsing).
   Context (sub_bytes:     bool -> state -> ident state)
           (shift_rows:    bool -> state -> ident state)
           (mix_columns:   bool -> state -> ident state)
-          (add_round_key : key -> state -> ident state).
+          (add_round_key : key -> state -> ident state)
+          (key_expand : bool -> round_index -> (key * round_constant) ->
+                        cava (key * round_constant)).
 
   Let sub_bytes' : state -> state := (fun st => unIdent (sub_bytes false st)).
   Let shift_rows' : state -> state := (fun st => unIdent (shift_rows false st)).
@@ -40,39 +65,289 @@ Section WithSubroutines.
   Let inv_sub_bytes' : state -> state := (fun st => unIdent (sub_bytes true st)).
   Let inv_shift_rows' : state -> state := (fun st => unIdent (shift_rows true st)).
   Let inv_mix_columns' : state -> state := (fun st => unIdent (mix_columns true st)).
-  (* Note: argument order is switched for spec *)
+  Let inv_mix_columns_key' : key * round_constant -> key * round_constant :=
+    (fun '(k, rcon) => (inv_mix_columns' k, rcon)).
+  (* Note: argument order of add_round_key is switched for spec *)
   Let add_round_key' : state -> key -> state :=
     (fun st k => unIdent (add_round_key k st)).
+  Let add_round_key'' : state -> key * round_constant -> state :=
+    (fun st '(k, _) => unIdent (add_round_key k st)).
+  Let key_expand' : nat -> key * round_constant -> key * round_constant :=
+    (fun round_i k_rcon => unIdent (key_expand false (nat_to_bitvec_sized 4 round_i) k_rcon)).
+  Let inv_key_expand' : nat -> key * round_constant -> key * round_constant :=
+    (fun round_i k_rcon => unIdent (key_expand true (nat_to_bitvec_sized 4 round_i) k_rcon)).
+
+  Local Ltac simplify_step :=
+    first [ destruct_pair_let
+          | rewrite N2Nat.id
+          | rewrite N2Bv_sized_Bv2N
+          | rewrite pairSel_mkpair
+          | progress simpl_ident ]; [ ].
+  Local Ltac simplify := repeat simplify_step.
+
+  (* key_expand_and_round is equivalent to interleaved cipher rounds
+     (excluding the final round) *)
+  Lemma key_expand_and_round_equiv
+        (key_rcon_data : key * round_constant * state)
+        add_round_key_in_sel round_key_sel
+        round_i :
+    let round := key_expand_and_round
+                   (round_index:=Vec Bit 4) (round_constant:=Vec Bit 8)
+                   sub_bytes shift_rows mix_columns add_round_key
+                   (mix_columns true)
+                   key_expand false in
+    let round_spec := cipher_round_interleaved
+                        add_round_key'' sub_bytes' shift_rows' mix_columns'
+                        key_expand' in
+    let i := N.to_nat (Bv2N round_i) in
+    add_round_key_in_sel = nat_to_bitvec_sized 2 (if Nat.eqb i 0 then 1 else 0) ->
+    round_key_sel = false ->
+    unIdent (round key_rcon_data add_round_key_in_sel round_key_sel round_i)
+    = round_spec key_rcon_data i.
+  Proof.
+    cbv zeta; intros. subst_lets. subst.
+    cbv [key_expand_and_round cipher_round cipher_round_interleaved mcompose].
+    cbv [nat_to_bitvec_sized].
+    destruct key_rcon_data as [[key rcon] data]. simplify.
+    rewrite <-surjective_pairing.
+    destruct_one_match;
+      compute_expr (nat_to_bitvec_sized 2 0);
+      compute_expr (nat_to_bitvec_sized 2 1).
+    all:rewrite mux4_mkpair; autorewrite with vsimpl.
+    all:reflexivity.
+  Qed.
+
+  (* key_expand_and_round is equivalent to (inverse) interleaved cipher rounds
+     (excluding the final round) *)
+  Lemma inverse_key_expand_and_round_equiv
+        (key_rcon_data : key * round_constant * state)
+        add_round_key_in_sel round_key_sel
+        round_i :
+    let round := key_expand_and_round
+                   (round_index:=Vec Bit 4) (round_constant:=Vec Bit 8)
+                   sub_bytes shift_rows mix_columns add_round_key
+                   (mix_columns true) key_expand true in
+    let round_spec := equivalent_inverse_cipher_round_interleaved
+                        add_round_key'' inv_sub_bytes' inv_shift_rows' inv_mix_columns'
+                        inv_key_expand' inv_mix_columns_key' in
+    let i := N.to_nat (Bv2N round_i) in
+    add_round_key_in_sel = nat_to_bitvec_sized 2 (if Nat.eqb i 0 then 1 else 0) ->
+    (* round_key_sel is true if this is a "middle round" (in this context, not round 0) *)
+    (round_key_sel = if Nat.eqb i 0 then false else true) ->
+    unIdent (round key_rcon_data add_round_key_in_sel round_key_sel round_i)
+    = round_spec key_rcon_data i.
+  Proof.
+    cbv zeta; intros. subst_lets. subst.
+    cbv [key_expand_and_round
+           cipher_round equivalent_inverse_cipher_round_interleaved mcompose].
+    cbv [nat_to_bitvec_sized]. destruct key_rcon_data as [[key rcon] data].
+    simplify.
+    repeat destruct_one_match; autorewrite with boolsimpl in *; try congruence.
+    all: compute_expr (N2Bv_sized 2 (N.of_nat 0)).
+    all: compute_expr (N2Bv_sized 2 (N.of_nat 1)).
+    all: rewrite mux4_mkpair; autorewrite with vsimpl.
+    all: rewrite <-surjective_pairing.
+    all: reflexivity.
+  Qed.
+
+  Lemma key_expand_and_round_last_equiv
+        is_decrypt (round_i : round_index) round_key rcon data :
+    snd (unIdent
+           (key_expand_and_round
+              (semantics:=CombinationalSemantics)
+              (round_index:=Vec Bit 4) (round_constant:=Vec Bit 8)
+              sub_bytes shift_rows mix_columns add_round_key (mix_columns true) key_expand
+              is_decrypt (round_key, rcon, data) [false; true] false round_i))
+    = if is_decrypt
+      then add_round_key' (inv_shift_rows' (inv_sub_bytes' data)) round_key
+      else add_round_key' (shift_rows' (sub_bytes' data)) round_key.
+  Proof.
+    cbv [key_expand_and_round mcompose]; intros. subst_lets.
+    simplify. rewrite mux4_mkpair. autorewrite with vsimpl.
+    destruct is_decrypt; reflexivity.
+  Qed.
 
   Lemma cipher_equiv
+        (Nr : nat) (init_rcon : round_constant) (round_indices : list round_index)
+        (num_regular_rounds round0 : round_index)
         (first_key last_key : key) (middle_keys : list key) (input : state) :
-    let cipher := (cipher sub_bytes shift_rows mix_columns add_round_key false) in
-    let cipher_spec := (Cipher.cipher _ _ add_round_key'
-                                      sub_bytes' shift_rows' mix_columns') in
-    unIdent (cipher first_key last_key middle_keys input)
-    = cipher_spec first_key last_key middle_keys input.
+    let all_keys_and_rcons := all_keys key_expand' Nr (first_key, init_rcon) in
+    let all_keys := List.map fst all_keys_and_rcons in
+    all_keys = (first_key :: middle_keys ++ [last_key])%list ->
+    (* Nr must be at least two and small enough to fit in round_index size *)
+    1 < Nr < 2 ^ 4 ->
+    round_indices = map (fun i => nat_to_bitvec_sized 4 i) (List.seq 0 (S Nr)) ->
+    num_regular_rounds = nat_to_bitvec_sized _ Nr ->
+    round0 = nat_to_bitvec_sized _ 0 ->
+    unIdent
+      (cipher
+         (round_index:=Vec Bit 4) (round_constant:=Vec Bit 8)
+         sub_bytes shift_rows mix_columns add_round_key (mix_columns true)
+         key_expand num_regular_rounds round0 false
+         first_key init_rcon round_indices input)
+    = Cipher.cipher
+        _ _ add_round_key' sub_bytes' shift_rows' mix_columns'
+        first_key last_key middle_keys input.
   Proof.
-    cbv zeta. subst sub_bytes' shift_rows' mix_columns' add_round_key'.
-    cbv [cipher cipher_round Cipher.cipher]. cbn [mcompose bind ret Monad_ident unIdent].
-    repeat (f_equal; [ ]). rewrite foldLM_ident_fold_left.
-    eapply fold_left_preserves_relation; [ reflexivity | ].
-    intros; subst. reflexivity.
+    cbv zeta; intro Hall_keys; intros. subst.
+    cbv [cipher cipher_step mcompose]. simplify.
+
+    (* Helpful rephrasing of Nr upper bound *)
+    assert (N.of_nat Nr < 2 ^ N.of_nat 4)%N
+      by (cbn; change (2^4)%nat with 16 in *; Lia.lia).
+    pose proof (N.size_nat_le 4 (N.of_nat Nr) ltac:(Lia.lia)).
+
+    (* simplify *)
+    cbn [unpeel nor2 and2 norBool andBool CombinationalSemantics
+                bind ret Monad_ident unIdent].
+
+    (* separate the last round *)
+    rewrite foldLM_ident_fold_left.
+    autorewrite with pull_snoc natsimpl.
+
+    (* simplify round-index comparisons *)
+    rewrite !eqb_nat_to_bitvec_sized, Nat.eqb_refl by Lia.lia.
+    match goal with |- context [?n =? 0] => destr (n =? 0); [ Lia.lia | ] end.
+    boolsimpl.
+
+    (* simplify expression within loop body and rephrase in terms of round spec *)
+    rewrite fold_left_map.
+    erewrite fold_left_ext_In.
+    2:{
+      intros *. intro Hin. apply in_seq in Hin.
+      autorewrite with natsimpl in *. repeat destruct_pair_let.
+      rewrite !eqb_nat_to_bitvec_sized by Lia.lia.
+      rewrite key_expand_and_round_equiv
+        by first [ boolsimpl; reflexivity
+                 | rewrite nat_to_bitvec_to_nat by Lia.lia;
+                   repeat destruct_one_match; (reflexivity || Lia.lia) ].
+      instantiate_app_by_reflexivity. }
+
+    (* Get all states from key expansion *)
+    map_inversion Hall_keys; subst.
+    match goal with H : @eq (list (_ * _)) _ (_ :: _ ++ [_])%list |- _ =>
+                    rename H into Hall_keys end.
+
+    (* representation change; use full key-expansion state (key * round_constant) *)
+    erewrite cipher_change_key_rep with (projkey:=@fst key round_constant)
+      by reflexivity.
+
+    erewrite <-cipher_interleaved_equiv by eassumption.
+    cbv [cipher_interleaved]. repeat destruct_pair_let.
+
+    (* rewrite last round in terms of subroutines *)
+    rewrite key_expand_and_round_last_equiv.
+
+    (* prove using loop invariant *)
+    factor_out_loops.
+    eapply fold_left_double_invariant_seq with (I:=fun _ x y => x = y).
+    { (* invariant holds at start of loop *)
+      reflexivity. }
+    { (* invariant holds through loop body *)
+      intros; subst. subst add_round_key''.
+      rewrite nat_to_bitvec_to_nat by Lia.lia.
+      cbv [cipher_round_interleaved].
+      repeat destruct_pair_let. subst_lets.
+      reflexivity. }
+    { (* invariant implies postcondition *)
+      intros; subst; reflexivity. }
+  Qed.
+
+  Lemma inv_mix_columns_key'_map keys :
+    map fst (map inv_mix_columns_key' keys) = map inv_mix_columns' (map fst keys).
+  Proof.
+    rewrite !map_map; apply map_ext.
+    intros; subst_lets. cbv beta.
+    repeat destruct_pair_let; reflexivity.
   Qed.
 
   Lemma inverse_cipher_equiv
+        (Nr : nat) (init_rcon : round_constant) (round_indices : list round_index)
+        (num_regular_rounds round0 : round_index)
         (first_key last_key : key) (middle_keys : list key) (input : state) :
-    let cipher := (cipher sub_bytes shift_rows mix_columns add_round_key true) in
-    let cipher_spec := (Cipher.equivalent_inverse_cipher
-                          _ _ add_round_key'
-                          inv_sub_bytes' inv_shift_rows' inv_mix_columns') in
-    unIdent (cipher first_key last_key middle_keys input)
-    = cipher_spec first_key last_key middle_keys input.
+    let all_keys_and_rcons := all_keys inv_key_expand' Nr (first_key, init_rcon) in
+    let all_keys := List.map fst all_keys_and_rcons in
+    all_keys = (first_key :: middle_keys ++ [last_key])%list ->
+    (* Nr must be at least two and small enough to fit in round_index size *)
+    1 < Nr < 2 ^ 4 ->
+    round_indices = map (fun i => nat_to_bitvec_sized 4 i) (List.seq 0 (S Nr)) ->
+    num_regular_rounds = nat_to_bitvec_sized _ Nr ->
+    round0 = nat_to_bitvec_sized _ 0 ->
+    unIdent
+      (cipher
+         (round_index:=Vec Bit 4) (round_constant:=Vec Bit 8)
+         sub_bytes shift_rows mix_columns add_round_key (mix_columns true)
+         key_expand num_regular_rounds round0 true
+         first_key init_rcon round_indices input)
+    = Cipher.equivalent_inverse_cipher
+        _ _ add_round_key' inv_sub_bytes' inv_shift_rows' inv_mix_columns'
+        first_key last_key (map inv_mix_columns' middle_keys) input.
   Proof.
-    cbv zeta. subst inv_sub_bytes' inv_shift_rows' inv_mix_columns' add_round_key'.
-    cbv [cipher cipher_round Cipher.equivalent_inverse_cipher].
-    cbn [mcompose bind ret Monad_ident unIdent].
-    repeat (f_equal; [ ]). rewrite foldLM_ident_fold_left.
-    eapply fold_left_preserves_relation; [ reflexivity | ].
-    intros; subst. reflexivity.
+    cbv zeta; intro Hall_keys; intros. subst.
+    cbv [cipher cipher_step mcompose]. simplify.
+
+    (* Helpful rephrasing of Nr upper bound *)
+    assert (N.of_nat Nr < 2 ^ N.of_nat 4)%N
+      by (cbn; change (2^4)%nat with 16 in *; Lia.lia).
+    pose proof (N.size_nat_le 4 (N.of_nat Nr) ltac:(Lia.lia)).
+
+    (* simplify *)
+    cbn [unpeel nor2 and2 norBool andBool CombinationalSemantics
+                bind ret Monad_ident unIdent].
+
+    (* separate the last round *)
+    rewrite foldLM_ident_fold_left.
+    autorewrite with pull_snoc natsimpl.
+
+    (* simplify round-index comparisons *)
+    rewrite !eqb_nat_to_bitvec_sized, Nat.eqb_refl by Lia.lia.
+    match goal with |- context [?n =? 0] => destr (n =? 0); [ Lia.lia | ] end.
+    boolsimpl.
+
+    (* simplify expression within loop body and rephrase in terms of round spec *)
+    rewrite fold_left_map.
+    erewrite fold_left_ext_In.
+    2:{
+      intros *. intro Hin. apply in_seq in Hin.
+      autorewrite with natsimpl in *. repeat destruct_pair_let.
+      rewrite !eqb_nat_to_bitvec_sized by Lia.lia.
+      rewrite inverse_key_expand_and_round_equiv
+        by first [ boolsimpl; reflexivity
+                 | rewrite nat_to_bitvec_to_nat by Lia.lia;
+                   repeat destruct_one_match; (reflexivity || Lia.lia) ].
+      instantiate_app_by_reflexivity. }
+
+    (* Extract information from key expansion expression *)
+    map_inversion Hall_keys. subst.
+    match goal with H : @eq (list (_ * _)) _ (_ :: _ ++ [_])%list |- _ =>
+                    rename H into Hall_keys end.
+
+    (* representation change; use full key-expansion state (key * round_constant) *)
+    erewrite equivalent_inverse_cipher_change_key_rep
+      with (projkey:=@fst key round_constant)
+           (middle_keys_alt:=List.map inv_mix_columns_key' _)
+      by (reflexivity || apply inv_mix_columns_key'_map).
+
+    erewrite <-equivalent_inverse_cipher_interleaved_equiv by eauto.
+    cbv [equivalent_inverse_cipher_interleaved].
+    repeat destruct_pair_let.
+
+    (* rewrite last round in terms of subroutines *)
+    rewrite key_expand_and_round_last_equiv.
+
+    (* prove using loop invariant *)
+    factor_out_loops.
+    eapply fold_left_double_invariant_seq with (I:=fun _ x y => x = y).
+    { (* invariant holds at start of loop *)
+      reflexivity. }
+    { (* invariant holds through loop body *)
+      intros; subst. subst add_round_key''.
+      rewrite nat_to_bitvec_to_nat by Lia.lia.
+      cbv [equivalent_inverse_cipher_round_interleaved].
+      repeat destruct_pair_let. subst_lets.
+      reflexivity. }
+    { (* invariant implies postcondition *)
+      intros; subst; reflexivity. }
   Qed.
+
 End WithSubroutines.
